tools/autocorres/WordAbstract.thy
@@ -370,12 +370,12 @@ lemma valid_typ_abs_fn_sint:
 
 lemma valid_typ_abs_fn_tuple:
   "\<lbrakk> valid_typ_abs_fn P_a Q_a abs_a conc_a; valid_typ_abs_fn P_b Q_b abs_b conc_b \<rbrakk> \<Longrightarrow>
-          valid_typ_abs_fn (\<lambda>(a, b). P_a a \<and> P_b b) (\<lambda>(a, b). Q_a a \<and> Q_b b) (map_pair abs_a abs_b) (map_pair conc_a conc_b)"
+          valid_typ_abs_fn (\<lambda>(a, b). P_a a \<and> P_b b) (\<lambda>(a, b). Q_a a \<and> Q_b b) (map_prod abs_a abs_b) (map_prod conc_a conc_b)"
   by clarsimp
 
 lemma introduce_typ_abs_fn_tuple:
   "\<lbrakk> introduce_typ_abs_fn abs_a; introduce_typ_abs_fn abs_b \<rbrakk> \<Longrightarrow>
-         introduce_typ_abs_fn (map_pair abs_a abs_b)"
+         introduce_typ_abs_fn (map_prod abs_a abs_b)"
   by clarsimp
 
 definition [simp]:
@@ -635,35 +635,35 @@ lemma corresTA_extract_preconds_of_call_final':
 lemma corresTA_prod_case:
  "\<lbrakk> introduce_typ_abs_fn rx1;
     introduce_typ_abs_fn rx2;
-    abstract_val (Q x) x (map_pair rx1 rx2) x';
+    abstract_val (Q x) x (map_prod rx1 rx2) x';
       \<And>a b a' b'. \<lbrakk> abs_var a rx1 a'; abs_var  b rx2 b' \<rbrakk>
                       \<Longrightarrow>  corresTA (P a b) rx ex (M a b) (M' a' b') \<rbrakk>  \<Longrightarrow>
     corresTA (\<lambda>s. case x of (a, b) \<Rightarrow> P a b s \<and> Q (a, b)) rx ex (case x of (a, b) \<Rightarrow> M a b) (case x' of (a, b) \<Rightarrow> M' a b)"
   apply clarsimp
   apply (rule corresXF_assume_pre)
-  apply (clarsimp simp: split_def map_pair_def)
+  apply (clarsimp simp: split_def map_prod_def)
   done
 
 lemma abstract_val_prod_case:
-  "\<lbrakk> abstract_val True r (map_pair f g) r';
+  "\<lbrakk> abstract_val True r (map_prod f g) r';
        \<And>a b a' b'. \<lbrakk>  abs_var a f a'; abs_var  b g b' \<rbrakk>
                      \<Longrightarrow> abstract_val (P a b) (M a b) h (M' a' b') \<rbrakk>
        \<Longrightarrow> abstract_val (P (fst r) (snd r))
             (case r of (a, b) \<Rightarrow> M a b) h
             (case r' of (a, b) \<Rightarrow> M' a b)"
   apply (case_tac r, case_tac r')
-  apply (clarsimp simp: map_pair_def)
+  apply (clarsimp simp: map_prod_def)
   done
 
 lemma abstract_val_prod_case_fun_app:
-  "\<lbrakk> abstract_val True r (map_pair f g) r';
+  "\<lbrakk> abstract_val True r (map_prod f g) r';
        \<And>a b a' b'. \<lbrakk>  abs_var a f a'; abs_var b g b' \<rbrakk>
                      \<Longrightarrow> abstract_val (P a b) (M a b s) h (M' a' b' s) \<rbrakk>
        \<Longrightarrow> abstract_val (P (fst r) (snd r))
             ((case r of (a, b) \<Rightarrow> M a b) s) h
             ((case r' of (a, b) \<Rightarrow> M' a b) s)"
   apply (case_tac r, case_tac r')
-  apply (clarsimp simp: map_pair_def)
+  apply (clarsimp simp: map_prod_def)
   done
 
 lemma abstract_val_of_nat:
@@ -677,7 +677,7 @@ lemma abstract_val_of_int:
 lemma abstract_val_tuple:
   "\<lbrakk> abstract_val P a absL a';
      abstract_val Q b absR b' \<rbrakk> \<Longrightarrow>
-         abstract_val (P \<and> Q) (a, b) (map_pair absL absR) (a', b')"
+         abstract_val (P \<and> Q) (a, b) (map_prod absL absR) (a', b')"
   by clarsimp
 
 lemma abstract_val_func:
