tools/c-parser/umm_heap/SepFrame.thy
@@ -16,7 +16,7 @@ begin
 
 class heap_state_type'
 
-classrel heap_state_type' < type
+instance heap_state_type' \<subseteq> type ..
 
 consts
   hst_mem :: "'a::heap_state_type' \<Rightarrow> heap_mem"
@@ -240,7 +240,7 @@ proof (rule, rule hoare_complete, simp only: valid_def, clarify)
       pre: "(P (f x) \<and>\<^sup>* R (h x)) (lift_hst x)"
   then obtain s\<^sub>0 and s\<^sub>1 where pre_P: "P (f x) s\<^sub>0" and pre_R: "R (h x) s\<^sub>1" and
       disj: "s\<^sub>0 \<bottom> s\<^sub>1" and m: "lift_hst x = s\<^sub>1 ++ s\<^sub>0"
-    by (clarsimp simp: sep_conj_def map_add_ac)
+    by (clarsimp simp: sep_conj_def map_ac_simps)
   with orig_spec hi_f have nofault: "\<not> exec_fatal C \<Gamma>
       (restrict_htd x (dom s\<^sub>0))"
     by (force simp: exec_fatal_def image_def lift_hst_def cvalid_def valid_def
